<?xml version="1.0" encoding="ISO-8859-1"?>
<rdf:RDF
    xmlns:rdf='http://www.w3.org/1999/02/22-rdf-syntax-ns#'
    xmlns:rdfs='http://www.w3.org/2000/01/rdf-schema#'
    xmlns:skos='http://www.w3.org/2004/02/skos/core#'
    xmlns:nt2='http://nasataxonomy.jpl.nasa.gov/cvFields#'
    xmlns:dcterms='http://purl.org/dc/terms/'
    xmlns:dc='http://purl.org/dc/elements/1.1/'>
 <skos:Concept rdf:about='nasa:access:13'>
  <skos:prefLabel>Patents and Intellectual Property</skos:prefLabel>
  <skos:broader rdf:resource='nasa:access:3'/>
  <skos:scopeNote>Information disclosing a new invention in which the Federal
    Government owns or may own a right, title, or interest.
  </skos:scopeNote>
  <nt2:status>Candidate</nt2:status>
  <nt2:type>Descriptor</nt2:type>
  <nt2:inputdate>2007-01-26</nt2:inputdate>
  <dcterms:dateAccepted>2007-01-26</dcterms:dateAccepted>
  <dcterms:modified>2007-01-27</dcterms:modified>
  <nt2:code>13</nt2:code>
 </skos:Concept>
 <skos:Concept rdf:about='nasa:access:4'>
  <skos:prefLabel>Public</skos:prefLabel>
  <skos:broader rdf:resource='nasa:access:1'/>
  <skos:scopeNote>Materials which have been reviewed and whose release to the
    public has been approved.
  </skos:scopeNote>
  <nt2:status>Approved</nt2:status>
  <nt2:type>Descriptor</nt2:type>
  <nt2:inputdate>2007-01-26</nt2:inputdate>
  <dcterms:dateAccepted>2007-01-26</dcterms:dateAccepted>
  <dcterms:modified>2007-01-27</dcterms:modified>
  <nt2:code>4</nt2:code>
 </skos:Concept>
 <skos:Concept rdf:about='nasa:access:10'>
  <skos:prefLabel>FOIA-exempt</skos:prefLabel>
  <skos:broader rdf:resource='nasa:access:3'/>
  <skos:scopeNote>Information originated within or furnished to NASA that
    falls under one or more of the exemption criteria of the
    Freedom of Information Act (5 U.S.C. §552). Other
    categories of SBU do not imply that the information has
    been determined to be exempt from disclosure under FOIA.
    Requests under FOIA, for information designated as SBU,
    will be reviewed and processed in the same manner as any
    other FOIA request.
  </skos:scopeNote>
  <nt2:status>Candidate</nt2:status>
  <nt2:type>Descriptor</nt2:type>
  <nt2:inputdate>2007-01-26</nt2:inputdate>
  <dcterms:dateAccepted>2007-01-26</dcterms:dateAccepted>
  <dcterms:modified>2007-01-26</dcterms:modified>
  <nt2:code>10</nt2:code>
 </skos:Concept>
 <skos:Concept rdf:about='nasa:access:11'>
  <skos:prefLabel>Export Controlled</skos:prefLabel>
  <skos:broader rdf:resource='nasa:access:3'/>
  <skos:scopeNote>Information subject to export control under the
    International Traffic in Arms Regulations (ITAR) or the
    Export Administration Regulations (EAR).
  </skos:scopeNote>
  <nt2:status>Candidate</nt2:status>
  <nt2:type>Descriptor</nt2:type>
  <nt2:inputdate>2007-01-26</nt2:inputdate>
  <dcterms:dateAccepted>2007-01-26</dcterms:dateAccepted>
  <dcterms:modified>2007-01-27</dcterms:modified>
  <nt2:code>11</nt2:code>
 </skos:Concept>
 <skos:Concept rdf:about='nasa:access:2'>
  <skos:prefLabel>Classified</skos:prefLabel>
  <skos:broader rdf:resource='nasa:access:1'/>
  <skos:narrower rdf:resource='nasa:access:6'/>
  <skos:narrower rdf:resource='nasa:access:7'/>
  <skos:narrower rdf:resource='nasa:access:8'/>
  <skos:scopeNote>Materials which have access controlled for reasons of
    national security. Materials should not be marked as
    "Classified", they must be marked according to the more
    specific classification levels of Confidential, Secret, or
    Top Secret.
    Classified materials must not be transferred to an
    unclassified system.
  </skos:scopeNote>
  <nt2:status>Approved</nt2:status>
  <nt2:type>Node label</nt2:type>
  <nt2:inputdate>2007-01-26</nt2:inputdate>
  <dcterms:dateAccepted>2007-01-26</dcterms:dateAccepted>
  <dcterms:modified>2007-01-27</dcterms:modified>
  <nt2:code>2</nt2:code>
 </skos:Concept>
 <skos:Concept rdf:about='nasa:access:3'>
  <skos:prefLabel>Sensitive But Unclassified</skos:prefLabel>
  <skos:altLabel>SBU</skos:altLabel>
  <skos:broader rdf:resource='nasa:access:1'/>
  <skos:narrower rdf:resource='nasa:access:11'/>
  <skos:narrower rdf:resource='nasa:access:10'/>
  <skos:narrower rdf:resource='nasa:access:17'/>
  <skos:narrower rdf:resource='nasa:access:12'/>
  <skos:narrower rdf:resource='nasa:access:13'/>
  <skos:narrower rdf:resource='nasa:access:16'/>
  <skos:narrower rdf:resource='nasa:access:14'/>
  <skos:narrower rdf:resource='nasa:access:15'/>
  <skos:scopeNote>Information, regardless of its form (digital, hard-copy,
    magnetic tape, etc.), the release of which could cause harm
    to a person's privacy or welfare, adversely impact economic
    or industrial institutions, or compromise programs or
    operations essential to the safeguarding of our national
    interests is designated as SBU to control or restrict its
    access. Information designated as SBU shall be afforded
    appropriate protection sufficient to safeguard it from
    unauthorized disclosure.
    Within NASA and the Federal Government, such information
    had previously been designated "FOR OFFICIAL USE ONLY."
    This designation was changed at NASA to "Administratively
    Controlled Information" for clarity and to more accurately
    describe the status of information to be protected.
    However, recent efforts to apply consistent terminology
    across multiple federal agencies have prompted NASA to
    change the designation to "Sensitive but Unclassified."
    Therefore the caveat "SENSITIVE BUT UNCLASSIFIED (SBU)"
    will be used to identify sensitive but unclassified
    information within the NASA community when that information
    is not otherwise specifically described and governed by
    statute or regulation. The use of caveats other than SBU
    will be governed by the statutes and regulations issued for
    the applicable category of information.
    (Source: NPR 1600.1 NASA Security Program Procedural
    Requirements, Section 5.2.4).
  </skos:scopeNote>
  <nt2:status>Approved</nt2:status>
  <nt2:type>Descriptor</nt2:type>
  <nt2:inputdate>2007-01-26</nt2:inputdate>
  <dcterms:dateAccepted>2007-01-26</dcterms:dateAccepted>
  <dcterms:modified>2007-01-26</dcterms:modified>
  <nt2:code>3</nt2:code>
 </skos:Concept>
 <skos:Concept rdf:about='nasa:access:6'>
  <skos:prefLabel>Confidential</skos:prefLabel>
  <skos:broader rdf:resource='nasa:access:2'/>
  <nt2:status>Approved</nt2:status>
  <nt2:type>Descriptor</nt2:type>
  <nt2:inputdate>2007-01-26</nt2:inputdate>
  <dcterms:dateAccepted>2007-01-26</dcterms:dateAccepted>
  <dcterms:modified>2007-01-27</dcterms:modified>
  <nt2:code>6</nt2:code>
 </skos:Concept>
 <skos:Concept rdf:about='nasa:access:5'>
  <skos:prefLabel>Unreviewed</skos:prefLabel>
  <skos:broader rdf:resource='nasa:access:1'/>
  <skos:scopeNote>Used to mark materials which have not been reviewed for
    relase to the public. Until they have been reviewed, the
    materials should be treated as Sensitive But Unclassified,
    with moderate levels of risk around compromise of their
    confidentiality, integrity, and availability.
  </skos:scopeNote>
  <nt2:status>Approved</nt2:status>
  <nt2:type>Descriptor</nt2:type>
  <nt2:inputdate>2007-01-26</nt2:inputdate>
  <dcterms:dateAccepted>2007-01-26</dcterms:dateAccepted>
  <dcterms:modified>2007-01-26</dcterms:modified>
  <nt2:code>5</nt2:code>
 </skos:Concept>
 <skos:Concept rdf:about='nasa:access:16'>
  <skos:prefLabel>Privacy Act</skos:prefLabel>
  <skos:broader rdf:resource='nasa:access:3'/>
  <skos:scopeNote>Information subject to the Privacy Act of 1974 (5 U.S.C.
    §552a).
  </skos:scopeNote>
  <nt2:status>Candidate</nt2:status>
  <nt2:type>Descriptor</nt2:type>
  <nt2:inputdate>2007-01-26</nt2:inputdate>
  <dcterms:modified>2007-01-27</dcterms:modified>
  <nt2:code>16</nt2:code>
 </skos:Concept>
 <skos:Concept rdf:about='nasa:access:17'>
  <skos:prefLabel>NASA Designated</skos:prefLabel>
  <skos:broader rdf:resource='nasa:access:3'/>
  <skos:scopeNote>Information that is determined by a designated NASA
    official to be unusually sensitive (refer to paragraph
    5.22.5. for decontrol provisions). The following are
    examples of such information.
    (1) Predecisional materials such as national space policy
    not yet publicly released, pending reorganization plans, or
    sensitive travel itineraries
    (2) Geological and geophysical information and data,
    including maps, concerning wells.
    (3) Center maps and/or plain text documents describing
    locations/directions (e.g., latitude, longitude, depth,
    etc.) of underground utility conduits (e.g., sewers, gas,
    data, communications, etc.).
    (4) Drawings and specifications that identify existing or
    proposed security measures for mission essential
    infrastructure designated assets or other key resources
    (5) Mission specific security plans that identify
    protective measures and procedures for assets that are
    sensitive in nature but are not classified. (Example:
    Payloads that utilize special nuclear materials, payloads
    that contain certain animal experiments, and STS missions,
    as determined by the CCS, etc.)
    (6) Emergency contingency or continuity of operations plans
    that provide detailed information regarding emergency
    response processes and procedures that, if publicized,
    could give a potential adversary vital information with
    which to thwart or compromise emergency response efforts.
    (7) Sensitive scientific and technical information (STI)
    (See NPD 2200.1 and NPR 2200.2 for requirements for
    documentation, approval, and dissemination of NASA STI).
    (8) Information that could result in physical risk to
    personnel.
    (9) NASA information technology (IT) internal systems data
    revealing infrastructure used for servers, desktops, and
    networks; applications name, version and release;
    switching, router, and gateway information;
    interconnections and access methods; mission or business
    use/need. Examples of information are systems inventories
    and enterprise architecture models.
    (10) Systems security data revealing the security posture
    of the system. For example, threat assessments, system
    security plans, contingency plans, risk management plans,
    Business Impact Analysis studies, and Certification and
    Accreditation documentation.
    (11) Reviews or reports illustrating or disclosing facility
    infrastructure or security vulnerabilities, whether to
    persons, systems, or facilities, not otherwise eligible for
    classification under Executive Order 12958, as amended.
    (12) Information that could constitute an indicator of U.S.
    government intentions, capabilities, operations, or
    activities or otherwise threaten operations security.
    (13) Developing or current technology, the release of which
    could hinder the objectives of NASA, compromise a
    technological advantage or countermeasure, cause a denial
    of service, or provide an adversary with sufficient
    information to clone, counterfeit, or circumvent a process
    or system.
  </skos:scopeNote>
  <nt2:status>Candidate</nt2:status>
  <nt2:type>Descriptor</nt2:type>
  <nt2:inputdate>2007-01-26</nt2:inputdate>
  <dcterms:modified>2007-01-27</dcterms:modified>
  <nt2:code>17</nt2:code>
 </skos:Concept>
 <skos:Concept rdf:about='nasa:access:15'>
  <skos:prefLabel>Space Act</skos:prefLabel>
  <skos:broader rdf:resource='nasa:access:3'/>
  <skos:scopeNote>Information developed by NASA under a Space Act agreement
    and subject to section 303(b) of the Space Act (42 U.S.C.
    2454(b)).
  </skos:scopeNote>
  <nt2:status>Candidate</nt2:status>
  <nt2:type>Descriptor</nt2:type>
  <nt2:inputdate>2007-01-26</nt2:inputdate>
  <dcterms:modified>2007-01-27</dcterms:modified>
  <nt2:code>15</nt2:code>
 </skos:Concept>
 <skos:Concept rdf:about='nasa:access:12'>
  <skos:prefLabel>Non-NASA Proprietary</skos:prefLabel>
  <skos:broader rdf:resource='nasa:access:3'/>
  <skos:scopeNote>Proprietary information of others provided to NASA under a
    nondisclosure or confidentiality agreement.
    
    Small Business Innovative Research Data, Limited Rights
    Data, and Restricted Computer Software received in
    performance of NASA contracts
    
    Information concerning or relating to private entity trade
    secrets or confidential commercial or financial information
    received by a NASA employee in the course of government
    employment or official duties.
  </skos:scopeNote>
  <nt2:status>Candidate</nt2:status>
  <nt2:type>Descriptor</nt2:type>
  <nt2:inputdate>2007-01-26</nt2:inputdate>
  <dcterms:dateAccepted>2007-01-26</dcterms:dateAccepted>
  <dcterms:modified>2007-01-27</dcterms:modified>
  <nt2:code>12</nt2:code>
 </skos:Concept>
 <skos:Concept rdf:about='nasa:access:8'>
  <skos:prefLabel>Top Secret</skos:prefLabel>
  <skos:broader rdf:resource='nasa:access:2'/>
  <nt2:status>Approved</nt2:status>
  <nt2:type>Descriptor</nt2:type>
  <nt2:inputdate>2007-01-26</nt2:inputdate>
  <dcterms:dateAccepted>2007-01-26</dcterms:dateAccepted>
  <dcterms:modified>2007-01-27</dcterms:modified>
  <nt2:code>8</nt2:code>
 </skos:Concept>
 <skos:Concept rdf:about='nasa:access:1'>
  <skos:prefLabel>Access Controls</skos:prefLabel>
  <skos:narrower rdf:resource='nasa:access:2'/>
  <skos:narrower rdf:resource='nasa:access:4'/>
  <skos:narrower rdf:resource='nasa:access:3'/>
  <skos:narrower rdf:resource='nasa:access:5'/>
  <skos:scopeNote>Based on NPR 1450.10D (for Classified) Section 8and NPR
    1600.1 (NASA Security Program Procedural Requirements),
    Section 5.24, and discussions with the NASA Taxonomy Team.
    
    This vocabulary is not intended for designing systems. It
    is intended to be used to mark individual information items
    so that their access can be controlled properly when they
    are moved between systems. For selecting the proper access
    controls when designing information systems, see NASA NPR
    2810 and NASA IS-SOP-0019B.
  </skos:scopeNote>
  <nt2:status>Approved</nt2:status>
  <nt2:type>Descriptor</nt2:type>
  <nt2:inputdate>2007-01-26</nt2:inputdate>
  <dcterms:dateAccepted>2007-01-26</dcterms:dateAccepted>
  <dcterms:modified>2007-01-26</dcterms:modified>
  <nt2:code>1</nt2:code>
 </skos:Concept>
 <skos:Concept rdf:about='nasa:access:14'>
  <skos:prefLabel>Procurement Sensitive</skos:prefLabel>
  <skos:broader rdf:resource='nasa:access:3'/>
  <skos:scopeNote>Source selection and bid and proposal information.
  </skos:scopeNote>
  <nt2:status>Candidate</nt2:status>
  <nt2:type>Descriptor</nt2:type>
  <nt2:inputdate>2007-01-26</nt2:inputdate>
  <dcterms:dateAccepted>2007-01-26</dcterms:dateAccepted>
  <dcterms:modified>2007-01-27</dcterms:modified>
  <nt2:code>14</nt2:code>
 </skos:Concept>
 <skos:Concept rdf:about='nasa:access:7'>
  <skos:prefLabel>Secret</skos:prefLabel>
  <skos:broader rdf:resource='nasa:access:2'/>
  <nt2:status>Approved</nt2:status>
  <nt2:type>Descriptor</nt2:type>
  <nt2:inputdate>2007-01-26</nt2:inputdate>
  <dcterms:dateAccepted>2007-01-26</dcterms:dateAccepted>
  <dcterms:modified>2007-01-27</dcterms:modified>
  <nt2:code>7</nt2:code>
 </skos:Concept>
</rdf:RDF>
